src/MinLTL.v
@@ -1,9 +1,9 @@
 Set Warnings "-local-declaration".
 
 Require Import
-  Coq.Classes.Equivalence
+  Coq.Program.Program
   Coq.Classes.Morphisms
-  Coq.Classes.SetoidClass
+  Coq.Setoids.Setoid
   Bool.
 
 (***********************************************************************
@@ -19,6 +19,10 @@ Module Type MinimalLinearTemporalLogic <: BooleanLogic.
 
 Include BooleanLogic.
 
+Parameters s : Type.
+
+Parameter holds : s -> nat -> t -> Prop.
+
 Parameter next : t -> t.
 Parameter until : t -> t -> t.
 
@@ -28,30 +32,46 @@ Delimit Scope ltl_scope with ltl.
 Open Scope boolean_scope.
 Open Scope ltl_scope.
 
-Notation "◯ p"     := (next p)    (at level 75, right associativity) : ltl_scope.
-Notation "p 'U' q" := (until p q) (at level 79, right associativity) : ltl_scope.
+Notation "[ σ , j ]  ⊨ p" := (holds σ j p) (at level 89, no associativity) : ltl_scope.
+Notation "◯ p"            := (next p)      (at level 75, right associativity) : ltl_scope.
+Notation "p 'U' q"        := (until p q)   (at level 79, right associativity) : ltl_scope.
 
-Declare Instance next_respects_impl : Proper (impl ==> impl) next.
-Declare Instance until_respects_impl : Proper (impl ==> impl ==> impl) until.
+Definition t_implies    p q := forall σ j, holds σ j (impl p q).
+Definition t_equivalent p q := t_implies p q /\ t_implies q p.
 
-Axiom (* 1 *) next_not : forall (p : t), ◯ ¬p ≈ ¬◯ p.
-Axiom (* 2 *) next_impl : forall (p q : t), ◯ (p ⇒ q) ≈ ◯ p ⇒ ◯ q.
+Declare Instance holds_respects_implies σ j :
+  Proper (implies ==> Basics.impl) (holds σ j).
+Declare Instance holds_respects_temporality σ j :
+  Proper ((fun p q => holds σ j (impl p q)) ==> Basics.impl) (holds σ j).
 
-Axiom (* 9 *) next_until : forall (p q : t), ◯ (p U q) ≈ (◯ p) U (◯ q).
-Axiom (* 10 *) until_expansion : forall (p q : t), p U q ≈ q ∨ (p ∧ ◯ (p U q)).
-Axiom (* 11 *) until_right_bottom : forall (p : t), p U ⊥ ≈ ⊥.
-Axiom (* 12 *) until_left_or : forall (p q r : t), p U (q ∨ r) ≈ (p U q) ∨ (p U r).
-Axiom (* 13 *) until_right_or : forall (p q r : t), (p U r) ∨ (q U r) ⟹ (p ∨ q) U r.
-Axiom (* 14 *) until_left_and : forall (p q r : t), p U (q ∧ r) ⟹ (p U q) ∧ (p U r).
-Axiom (* 15 *) until_right_and : forall (p q r : t), (p ∧ q) U r ≈ (p U r) ∧ (q U r).
-Axiom (* 16 *) until_impl_order : forall (p q r : t), (p U q) ∧ (¬q U r) ⟹ p U r.
-Axiom (* 17 *) until_right_or_order : forall (p q r : t), p U (q U r) ⟹ (p ∨ q) U r.
-Axiom (* 18 *) until_right_and_order : forall (p q r : t), p U (q ∧ r) ⟹ (p U q) U r.
+Declare Instance next_respects_implies : Proper (implies ==> implies) next.
+Declare Instance until_respects_implies : Proper (implies ==> implies ==> implies) until.
+
+Infix "⟹" := t_implies    (at level 99, right associativity) : ltl_scope.
+Infix "≈"  := t_equivalent (at level 90, no associativity) : ltl_scope.
+
+Axiom truth_holds : forall p, truth p <-> forall σ j, holds σ j p.
+
+Axiom next_semantics : forall σ j p, [σ, j] ⊨ ◯ p <-> [σ, j + 1] ⊨ p.
+
+Axiom (* 1 *)  next_not : forall p, ◯ ¬p ≈ ¬◯ p.
+Axiom (* 2 *)  next_impl : forall p q, ◯ (p ⇒ q) ≈ ◯ p ⇒ ◯ q.
+
+Axiom (* 9 *)  next_until : forall p q, ◯ (p U q) ≈ (◯ p) U (◯ q).
+Axiom (* 10 *) until_expansion : forall p q, p U q ≈ q ∨ (p ∧ ◯ (p U q)).
+Axiom (* 11 *) until_right_bottom : forall p, p U ⊥ ≈ ⊥.
+Axiom (* 12 *) until_left_or : forall p q r, p U (q ∨ r) ≈ (p U q) ∨ (p U r).
+Axiom (* 13 *) until_right_or : forall p q r, (p U r) ∨ (q U r) ⟹ (p ∨ q) U r.
+Axiom (* 14 *) until_left_and : forall p q r, p U (q ∧ r) ⟹ (p U q) ∧ (p U r).
+Axiom (* 15 *) until_right_and : forall p q r, (p ∧ q) U r ≈ (p U r) ∧ (q U r).
+Axiom (* 16 *) until_impl_order : forall p q r, (p U q) ∧ (¬q U r) ⟹ p U r.
+Axiom (* 17 *) until_right_or_order : forall p q r, p U (q U r) ⟹ (p ∨ q) U r.
+Axiom (* 18 *) until_right_and_order : forall p q r, p U (q ∧ r) ⟹ (p U q) U r.
 
 (** jww (2021-02-08): This axiom is just an idea a work in progress *)
-(* Axiom (* NEW *) until_continue : forall (p q : t), q ∧ p U ◯ ¬q ⟹ p U (q ∧ ◯ ¬q). *)
-Axiom (* NEW *) always_until : forall (p q r : t), ¬(⊤ U ¬p) ∧ q U r ≈ (p ∧ q) U (p ∧ r).
-Axiom (* NEW *) not_until    : forall (p q : t), ⊤ U ¬p ∧ ¬(p U q) ≈ ¬q U (¬p ∧ ¬q).
+(* Axiom (* NEW *) until_continue : forall p q, q ∧ p U ◯ ¬q ⟹ p U (q ∧ ◯ ¬q). *)
+Axiom (* NEW *) always_until : forall p q r, ¬(⊤ U ¬p) ∧ q U r ≈ (p ∧ q) U (p ∧ r).
+Axiom (* NEW *) not_until    : forall p q, ⊤ U ¬p ∧ ¬(p U q) ≈ ¬q U (¬p ∧ ¬q).
 
 End MinimalLinearTemporalLogic.
 
@@ -61,8 +81,274 @@ Import L.
 Module Import BF := BooleanLogicFacts L.
 Module Import MBF := BF.MBF.
 
-Program Instance next_respects_eqv : Proper (eqv ==> eqv) next.
-Program Instance until_respects_eqv : Proper (eqv ==> eqv ==> eqv) until.
+Lemma t_impl p q : (p ⟹ q)%boolean <-> (p ⟹ q).
+Proof.
+  unfold t_implies.
+  split; intro H.
+  - apply truth_holds.
+    now apply H.
+  - apply truth_holds in H.
+    now apply H.
+Qed.
+
+Lemma t_eqv p q : (p ≈ q)%boolean <-> p ≈ q.
+Proof.
+  unfold t_equivalent.
+  split; intro H.
+  - destruct H.
+    split; now apply t_impl.
+  - destruct H.
+    split; now apply t_impl.
+Qed.
+
+Program Instance next_respects_equivalent :
+  Proper (equivalent ==> equivalent) next.
+Program Instance until_respects_equivalent :
+  Proper (equivalent ==> equivalent ==> equivalent) until.
+
+Local Obligation Tactic := program_simpl.
+
+Program Instance t_implies_reflexive : Reflexive t_implies.
+Next Obligation.
+  unfold t_implies; intros.
+  apply truth_holds.
+  reflexivity.
+Qed.
+
+Program Instance t_implies_transitive : Transitive t_implies.
+Next Obligation.
+  unfold t_implies in *; intros.
+  apply truth_holds in H.
+  apply truth_holds in H0.
+  apply truth_holds.
+  now transitivity y.
+Qed.
+
+Program Instance t_equivalent_Equivalence : Equivalence t_equivalent.
+Next Obligation. now intro x; split. Qed.
+Next Obligation. repeat intro; split; destruct H; now intuition. Qed.
+Next Obligation. repeat intro; split; destruct H, H0; now transitivity y. Qed.
+
+Arguments holds_respects_temporality {_ _ _ _} H.
+
+Program Instance holds_respects_t_implies σ j :
+  Proper (t_implies ==> Basics.impl) (holds σ j).
+Next Obligation.
+  repeat intro.
+  now apply (holds_respects_temporality (H σ j)).
+Qed.
+
+Program Instance holds_respects_equivalent σ j :
+  Proper (equivalent ==> iff) (holds σ j).
+Next Obligation.
+  repeat intro.
+  destruct H.
+  split; intro.
+  - unfold implies in H.
+    pose proof (proj1 (truth_holds _) H).
+    now apply (holds_respects_temporality (H2 σ j)).
+  - unfold implies in H0.
+    pose proof (proj1 (truth_holds _) H0).
+    now apply (holds_respects_temporality (H2 σ j)).
+Qed.
+
+Program Instance holds_respects_t_equivalent σ j :
+  Proper (t_equivalent ==> iff) (holds σ j).
+Next Obligation.
+  repeat intro.
+  destruct H.
+  split; intro.
+  - now rewrite <- H.
+  - now rewrite <- H0.
+Qed.
+
+Program Instance t_implies_respects_implies :
+  Proper (implies --> implies ==> Basics.impl) t_implies.
+Next Obligation.
+  repeat intro.
+  unfold Basics.flip in H.
+  apply truth_holds in H1.
+  revert j.
+  revert σ.
+  apply truth_holds.
+  now rewrite H, <- H0.
+Qed.
+
+Program Instance t_implies_respects_t_implies :
+  Proper (t_implies --> t_implies ==> Basics.impl) t_implies.
+Next Obligation.
+  repeat intro.
+  unfold Basics.flip in H.
+  apply truth_holds in H.
+  apply truth_holds in H0.
+  apply truth_holds in H1.
+  revert j.
+  revert σ.
+  apply truth_holds.
+  now rewrite H, <- H0.
+Qed.
+
+Program Instance t_implies_respects_equivalent :
+  Proper (equivalent ==> equivalent ==> iff) t_implies.
+Next Obligation.
+  repeat intro.
+  destruct H, H0.
+  split; intros.
+  - now rewrite H1, H3, H0.
+  - now rewrite <- H2, <- H3, <- H.
+Qed.
+
+Program Instance t_implies_respects_t_equivalent :
+  Proper (t_equivalent ==> t_equivalent ==> iff) t_implies.
+Next Obligation.
+  repeat intro.
+  destruct H, H0.
+  split; intros.
+  - now rewrite H1, H3, H0.
+  - now rewrite <- H2, <- H3, <- H.
+Qed.
+
+Program Instance t_equivalent_respects_equivalent :
+  Proper (equivalent ==> equivalent ==> iff) t_equivalent.
+Next Obligation.
+  repeat intro.
+  destruct H, H0.
+  split; intros.
+  - split; intros.
+    + destruct H3.
+      now rewrite H1, H3, H0.
+    + destruct H3.
+      now rewrite H2, H4, H.
+  - split; intros.
+    + destruct H3.
+      now rewrite H, H3, H2.
+    + destruct H3.
+      now rewrite H0, H4, H1.
+Qed.
+
+Program Instance t_equivalent_respects_t_equivalent :
+  Proper (t_equivalent ==> t_equivalent ==> iff) t_equivalent.
+Next Obligation.
+  repeat intro.
+  destruct H, H0.
+  split; intros.
+  - split; intros.
+    + destruct H3.
+      now rewrite H1, H3, H0.
+    + destruct H3.
+      now rewrite H2, H4, H.
+  - split; intros.
+    + destruct H3.
+      now rewrite H, H3, H2.
+    + destruct H3.
+      now rewrite H0, H4, H1.
+Qed.
+
+Program Instance impl_respects_t_implies :
+  Proper (t_implies --> t_implies ==> t_implies) impl.
+Next Obligation.
+  repeat intro.
+  apply truth_holds in H.
+  apply truth_holds in H0.
+  apply truth_holds.
+  rewrite <- H.
+  rewrite H0.
+  reflexivity.
+Qed.
+
+Program Instance impl_respects_t_equivalent :
+  Proper (t_equivalent ==> t_equivalent ==> t_equivalent) impl.
+Next Obligation.
+  repeat intro.
+  destruct H, H0.
+  split; intros.
+  + now rewrite <- H1, H0.
+  + now rewrite <- H, H2.
+Qed.
+
+Program Instance not_respects_t_implies : Proper (t_implies --> t_implies) not.
+Next Obligation.
+  repeat intro.
+  unfold flip in H.
+  apply truth_holds in H.
+  apply truth_holds.
+  now rewrite H.
+Qed.
+
+Program Instance not_respects_t_equivalent :
+  Proper (t_equivalent ==> t_equivalent) not.
+Next Obligation.
+  repeat intro.
+  destruct H.
+  split; intros.
+  - now rewrite H0.
+  - now rewrite H.
+Qed.
+
+Program Instance or_respects_t_implies :
+  Proper (t_implies ==> t_implies ==> t_implies) or.
+Next Obligation.
+  repeat intro.
+  apply truth_holds in H.
+  apply truth_holds in H0.
+  apply truth_holds.
+  now rewrite H, H0.
+Qed.
+
+Program Instance or_respects_t_equivalent :
+  Proper (t_equivalent ==> t_equivalent ==> t_equivalent) or.
+Next Obligation.
+  repeat intro.
+  destruct H, H0.
+  split; intros.
+  - now rewrite H, H0.
+  - now rewrite H1, H2.
+Qed.
+
+Program Instance and_respects_t_implies :
+  Proper (t_implies ==> t_implies ==> t_implies) and.
+Next Obligation.
+  repeat intro.
+  apply truth_holds in H.
+  apply truth_holds in H0.
+  apply truth_holds.
+  now rewrite H, H0.
+Qed.
+
+Program Instance and_respects_t_equivalent :
+  Proper (t_equivalent ==> t_equivalent ==> t_equivalent) and.
+Next Obligation.
+  repeat intro.
+  destruct H, H0.
+  split; intros.
+  - now rewrite H, H0.
+  - now rewrite H1, H2.
+Qed.
+
+Program Instance next_respects_t_implies :
+  Proper (t_implies ==> t_implies) next.
+Next Obligation.
+  repeat intro.
+  rewrite <- next_impl.
+  rewrite next_semantics.
+  now apply H.
+Qed.
+
+Program Instance next_respects_t_equivalent :
+  Proper (t_equivalent ==> t_equivalent) next.
+Next Obligation.
+  repeat intro.
+  destruct H.
+  split; intros.
+  - now rewrite <- H.
+  - now rewrite <- H0.
+Qed.
+
+Program Instance until_respects_t_implies :
+  Proper (t_implies ==> t_implies ==> t_implies) until.
+
+Program Instance until_respects_t_equivalent :
+  Proper (t_equivalent ==> t_equivalent ==> t_equivalent) until.
 
 (*** 3.1 Next ◯ *)
 
@@ -77,20 +363,22 @@ Program Instance until_respects_eqv : Proper (eqv ==> eqv ==> eqv) until.
 (8) Falsehood of ◯ : ◯ false ≡ false
 *)
 
-Theorem (* 3 *) next_linearity (p : t) : ◯ p ≈ ¬◯ ¬p.
+Theorem (* 3 *) next_linearity p : ◯ p ≈ ¬◯ ¬p.
 Proof.
   rewrite next_not.
-  now apply not_swap.
+  now rewrite not_not.
 Qed.
 
-Theorem (* 4 *) next_or (p q : t) : ◯ (p ∨ q) ≈ ◯ p ∨ ◯ q.
+Theorem (* 4 *) next_or p q : ◯ (p ∨ q) ≈ ◯ p ∨ ◯ q.
 Proof.
-  pose proof (next_impl (¬p) q) as H; rewrite not_not in H.
+  pose proof (next_impl (¬p) q) as H.
+  rewrite !impl_def in H.
+  rewrite not_not in H.
   rewrite H.
   now rewrite <- next_linearity.
 Qed.
 
-Theorem (* 5 *) next_and (p q : t) : ◯ (p ∧ q) ≈ ◯ p ∧ ◯ q.
+Theorem (* 5 *) next_and p q : ◯ (p ∧ q) ≈ ◯ p ∧ ◯ q.
 Proof.
   rewrite <- (not_not p) at 1.
   rewrite <- (not_not q) at 1.
@@ -101,11 +389,16 @@ Proof.
   now rewrite <- !next_linearity.
 Qed.
 
-Theorem (* 6 *) next_eqv (p q : t) : ◯ (p ≡ q) ≈ ◯ p ≡ ◯ q.
+Notation "p ≡ q" := (¬(¬(p ⇒ q) ∨ ¬(p ⇒ q))) (at level 86, right associativity) : boolean_scope.
+
+Theorem (* 6 *) next_eqv p q : ◯ (p ≡ q) ≈ ◯ p ≡ ◯ q.
 Proof.
-  rewrite !next_or.
-  rewrite !next_not.
-  now rewrite next_and.
+  rewrite !impl_def.
+  rewrite <- !next_not.
+  rewrite <- !next_or.
+  rewrite <- !next_not.
+  rewrite <- !next_or.
+  now rewrite <- !next_not.
 Qed.
 
 Theorem (* 7 *) next_true : ◯ ⊤ ≈ ⊤.
@@ -159,7 +452,7 @@ Qed.
 (37) Right absorption of U : (p U q) U q ≡ p U q
 *)
 
-Theorem (* 19 *) until_right_impl (p q r : t) : (p ⇒ q) U r ⟹ (p U r) ⇒ (q U r).
+Theorem (* 19 *) until_right_impl p q r : (p ⇒ q) U r ⟹ (p U r) ⇒ (q U r).
 Proof.
   apply and_impl_iff.
   rewrite <- until_right_and.
@@ -170,33 +463,33 @@ Proof.
   now apply and_proj.
 Qed.
 
-Theorem (* 20 *) until_true (p : t) : p U ⊤ ≈ ⊤.
+Theorem (* 20 *) until_true p : p U ⊤ ≈ ⊤.
 Proof.
   rewrite until_expansion.
   now rewrite true_or.
 Qed.
 
-Theorem (* 21 *) false_until (p : t) : ⊥ U p ≈ p.
+Theorem (* 21 *) false_until p : ⊥ U p ≈ p.
 Proof.
   rewrite until_expansion.
   rewrite false_and.
   now rewrite or_false.
 Qed.
 
-Theorem (* 22 *) until_idem (p : t) : p U p ≈ p.
+Theorem (* 22 *) until_idem p : p U p ≈ p.
 Proof.
   rewrite until_expansion.
   now rewrite or_absorb.
 Qed.
 
-Theorem (* 23 *) until_excl_middle (p q : t) : (p U q) ∨ (p U ¬q) ≈ ⊤.
+Theorem (* 23 *) until_excl_middle p q : (p U q) ∨ (p U ¬q) ≈ ⊤.
 Proof.
   rewrite <- until_left_or.
   rewrite true_def.
   now apply until_true.
 Qed.
 
-Theorem (* 24 *) until_24 (p q r : t) : (¬p U (q U r)) ∧ (p U r) ⟹ q U r.
+Theorem (* 24 *) until_24 p q r : (¬p U (q U r)) ∧ (p U r) ⟹ q U r.
 Proof.
   rewrite until_right_or_order.
   rewrite until_right_impl.
@@ -205,7 +498,7 @@ Proof.
   now boolean.
 Qed.
 
-Theorem (* 25 *) until_25 (p q r : t) : (p U (¬q U r)) ∧ (q U r) ⟹ p U r.
+Theorem (* 25 *) until_25 p q r : (p U (¬q U r)) ∧ (q U r) ⟹ p U r.
 Proof.
   rewrite until_right_or_order.
   rewrite or_comm.
@@ -215,13 +508,13 @@ Proof.
   now boolean.
 Qed.
 
-Theorem (* 26 *) until_26 (p q : t) : (p U q) ∧ (¬q U p) ⟹ p.
+Theorem (* 26 *) until_26 p q : (p U q) ∧ (¬q U p) ⟹ p.
 Proof.
   rewrite until_impl_order.
   now rewrite until_idem.
 Qed.
 
-Theorem (* 27 *) until_27 (p q : t) : p ∧ (¬p U q) ⟹ q.
+Theorem (* 27 *) until_27 p q : p ∧ (¬p U q) ⟹ q.
 Proof.
   rewrite until_expansion.
   rewrite and_or.
@@ -229,7 +522,7 @@ Proof.
   now boolean.
 Qed.
 
-Theorem (* 28 *) until_28 (p q : t) : p U q ⟹ p ∨ q.
+Theorem (* 28 *) until_28 p q : p U q ⟹ p ∨ q.
 Proof.
   rewrite until_expansion.
   rewrite or_and.
@@ -237,13 +530,13 @@ Proof.
   now rewrite or_comm.
 Qed.
 
-Theorem (* 29 *) until_insertion (p q : t) : q ⟹ p U q.
+Theorem (* 29 *) until_insertion p q : q ⟹ p U q.
 Proof.
   rewrite until_expansion.
   now apply or_inj.
 Qed.
 
-Theorem (* 30 *) until_30 (p q : t) : p ∧ q ⟹ p U q.
+Theorem (* 30 *) until_30 p q : p ∧ q ⟹ p U q.
 Proof.
   rewrite until_expansion.
   rewrite <- or_inj.
@@ -251,7 +544,7 @@ Proof.
   now apply and_proj.
 Qed.
 
-Theorem (* 31 *) until_absorb_or_u (p q : t) : p ∨ (p U q) ≈ p ∨ q.
+Theorem (* 31 *) until_absorb_or_u p q : p ∨ (p U q) ≈ p ∨ q.
 Proof.
   split.
   - rewrite (until_28 p q) at 1.
@@ -260,7 +553,7 @@ Proof.
   - now rewrite <- until_insertion.
 Qed.
 
-Theorem (* 32 *) until_absorb_u_or (p q : t) : (p U q) ∨ q ≈ p U q.
+Theorem (* 32 *) until_absorb_u_or p q : (p U q) ∨ q ≈ p U q.
 Proof.
   rewrite until_expansion.
   rewrite or_comm at 1.
@@ -268,7 +561,7 @@ Proof.
   now rewrite or_idem.
 Qed.
 
-Theorem (* 33 *) until_absorb_u_and (p q : t) : (p U q) ∧ q ≈ q.
+Theorem (* 33 *) until_absorb_u_and p q : (p U q) ∧ q ≈ q.
 Proof.
   split.
   - rewrite and_comm.
@@ -277,7 +570,7 @@ Proof.
     now rewrite (until_insertion p q) at 1.
 Qed.
 
-Theorem (* 34 *) until_absorb_u_or_and (p q : t) : (p U q) ∨ (p ∧ q) ≈ p U q.
+Theorem (* 34 *) until_absorb_u_or_and p q : (p U q) ∨ (p ∧ q) ≈ p U q.
 Proof.
   split.
   - rewrite until_30.
@@ -285,7 +578,7 @@ Proof.
   - now rewrite <- or_inj.
 Qed.
 
-Theorem (* 35 *) until_absorb_u_and_or (p q : t) : (p U q) ∧ (p ∨ q) ≈ p U q.
+Theorem (* 35 *) until_absorb_u_and_or p q : (p U q) ∧ (p ∨ q) ≈ p U q.
 Proof.
   split.
   - now apply and_proj.
@@ -293,7 +586,7 @@ Proof.
     now rewrite and_idem.
 Qed.
 
-Theorem (* 36 *) until_left_absorb (p q : t) : p U (p U q) ≈ p U q.
+Theorem (* 36 *) until_left_absorb p q : p U (p U q) ≈ p U q.
 Proof.
   split.
   - rewrite until_right_or_order.
@@ -301,7 +594,7 @@ Proof.
   - now apply until_insertion.
 Qed.
 
-Theorem (* 37 *) until_right_absorb (p q : t) : (p U q) U q ≈ p U q.
+Theorem (* 37 *) until_right_absorb p q : (p U q) U q ≈ p U q.
 Proof.
   split.
   - rewrite until_28.
@@ -310,7 +603,7 @@ Proof.
     now rewrite and_idem.
 Qed.
 
-Theorem (* NEW *) until_left_and_impl (p q r : t) : p U q ∧ p U r ⟹ p U (q ∨ r).
+Theorem (* NEW *) until_left_and_impl p q r : p U q ∧ p U r ⟹ p U (q ∨ r).
 Proof.
   rewrite until_left_or.
   rewrite and_proj.
